dsubsup_total_rec_monotone.v: many changes
* Start defining a variant of val_type in pieces, and strengthen obligation
  tactics to solve new, more varied Program obligations.
* Revise hints and tactics:
  + Hint for `lexprod`;
  + Hint Extern for `tsize_flat`;
  + Better `discriminatePlus`;
  + Use `open_preserves_size'`.
  + Make `valTypeObligationsSSReflection` the default program tactic (locally).
  + Readd `omega` to `simple_ineq`.
* Move/comment out unused definitions (nvset, mon_nvset).

ecoop17/dsubsup_total_rec_monotone.v
@@ -21,24 +21,21 @@ Require Import Coq.Wellfounded.Lexicographic_Product.
 I'm changing definitions a lot to make val_type monotone.
 *)
 
+Hint Constructors lexprod.
+
 Definition val_type_measure T (k : nat) := (existT (fun _ => nat) k (tsize_flat T)).
 
 Hint Unfold val_type_measure.
 
 Definition vset := vl -> Prop.
 Hint Unfold vset.
-Definition nvset := nat -> vset.
-Hint Unfold nvset.
-
-Definition mon_nvset := { phi : nvset | forall m n v, m < n -> phi n v -> phi m v }.
-Hint Unfold mon_nvset.
 
 Definition termRel := lexprod nat (fun _ => nat) lt (fun _ => lt).
 Hint Unfold termRel.
 
 Lemma wf_termRel : well_founded termRel.
 Proof.
- apply wf_lexprod; try intro; apply lt_wf.
+ apply wf_lexprod; intro; apply lt_wf.
 Defined.
 Hint Resolve wf_termRel.
 
@@ -57,6 +54,286 @@ Hint Resolve wf_val_type_termRel.
 (* Program Fixpoint val_type (env: list vseta) (GH:list vseta) (T:ty) n (dd: vset n) (v:vl) {measure (tsize_flat T)}: Prop := *)
 
 Global Unset Transparent Obligations.
+
+(* Show that different branches are disjoint. *)
+Ltac discriminatePlus :=
+  (* repeat split; intros; let Habs := fresh "Habs" in intro Habs; destruct Habs; discriminate. *)
+  repeat split_conj; intros;
+  (let Habs := fresh "Habs" in
+  try (intro Habs; destruct Habs) + idtac);
+  discriminate.
+
+(* Prove some inequalities needed below, without producing big proof terms like omega does. Probably not worth it. *)
+Ltac simple_ineq :=
+  (* simpl; omega. *)
+  simpl; auto using le_n_S, le_plus_l, le_plus_r; omega.
+  (* If this tactic fails, add back omega at the end. *)
+
+Hint Extern 5 (_ < tsize_flat _) =>
+  unfold open;
+  rewrite open_preserves_size';
+  simple_ineq.
+
+(* These three lemmas take care of the various forms of proof obligations that arise from val_type. *)
+Lemma termRelShow: forall j n T1 T2,
+  j <= n -> tsize_flat T2 < tsize_flat T1 ->
+  val_type_termRel (T2, j) (T1, n).
+Proof.
+  intros * Hj Ht.
+  unfold val_type_termRel, MR, termRel, argMeasure, val_type_measure.
+  (* If we only know that Hj: j <= n, we must case-split on it, and use
+     smaller_types when j = n and smaller_n when j < n. *)
+  destruct Hj; try assert (j < S m) by simple_ineq; auto.
+Qed.
+  (* - apply right_lex. assumption. *)
+  (* - apply left_lex. omega. *)
+
+
+Lemma termRelShowOpen: forall j n x T1 T2,
+  j <= n -> tsize_flat T2 < tsize_flat T1 ->
+  val_type_termRel (open (varH x) T2, j) (T1, n).
+Proof.
+  intros * Hj Ht.
+  unfold val_type_termRel, MR, termRel, argMeasure, val_type_measure.
+  destruct Hj; try assert (j < S m) by simple_ineq; auto.
+  (* unfold open; try rewrite open_preserves_size'. *)
+  (* auto using left_lex, right_lex. *)
+Qed.
+
+Lemma termRelShowLt: forall j n T1 T2,
+  j < n ->
+  val_type_termRel (T2, j) (T1, n).
+Proof.
+  intros * Hj.
+  unfold val_type_termRel, MR, termRel, argMeasure, val_type_measure.
+  auto.
+Qed.
+
+Ltac applyNSimpleIneq l := apply l; simple_ineq.
+
+Ltac smaller_n :=
+  Tactics.program_simpl;
+  autounfold; apply left_lex;
+  (* simpl; omega. *)
+  simple_ineq.
+
+Ltac smaller_types :=
+  Tactics.program_simpl;
+  autounfold; apply right_lex;
+  unfold open; try rewrite open_preserves_size';
+  (* simpl; omega. *)
+  simple_ineq.
+
+(* Solve obligations from valType using ssreflect-based ideas, that is, reusing lemmas for the various cases. *)
+Ltac valTypeObligationsSSReflection :=
+  program_simpl;
+  try solve [simple_ineq | applyNSimpleIneq termRelShowOpen | applyNSimpleIneq termRelShow | applyNSimpleIneq termRelShowLt | smaller_types | discriminatePlus].
+
+Local Obligation Tactic := valTypeObligationsSSReflection.
+
+Ltac valTypeObligations Hj :=
+  Tactics.program_simpl;
+  solve [ smaller_n | smaller_types | discriminatePlus | (try destruct Hj; [ smaller_types | smaller_n ])].
+
+(* Definition nvset := nat -> vset. *)
+(* Hint Unfold nvset. *)
+
+(* Definition mon_nvset := { phi : nvset | forall m n v, m < n -> phi n v -> phi m v }. *)
+(* Hint Unfold mon_nvset. *)
+
+Definition type_dom n :=
+  list vl -> list vl -> vl ->
+  forall (n0: nat) (H: n0 <= n), Prop.
+Hint Unfold type_dom.
+
+Definition smaller_args T0 n0 T n :=
+  termRel (val_type_measure T0 n0) (val_type_measure T n).
+Hint Unfold smaller_args.
+
+Definition type_dom2 T n :=
+  forall (T0 : ty),
+    list vl -> list vl -> vl ->
+    forall (n0: nat) (Hle : smaller_args T0 n0 T n), Prop.
+
+Program Definition expr_sem {n} (A : type_dom n) :=
+  fun env env1 GH e j p =>
+        exists v, tevaln env1 e v /\
+                  A env GH v j p.
+
+Program Definition conv {T} {n} (A: type_dom2 T n) T1 (H: tsize_flat T1 < tsize_flat T): type_dom n :=
+  fun env GH v n p => A T1 env GH v n _.
+Hint Unfold conv.
+
+Program Definition interpTAll n
+        (A1 : type_dom n)
+        (A2 : type_dom n)
+  : type_dom n :=
+  fun env GH v n0 p =>
+    match v with
+    | vabs env1 T0 t =>
+      forall vx j (Hj: j <= n0),
+        A1 env GH vx j _ ->
+        expr_sem A2 env (vx :: env1) (vx :: GH) t j _
+        (* exists v, tevaln (vx::env1) y v /\ *)
+        (*           B env (vx::GH) j v *)
+    | _ => False
+    end.
+Hint Unfold interpTAll.
+
+(* Solve Obligations with Tactics.program_simpl; simple_ineq. *)
+(* Solve Obligations with valTypeObligationsSSReflection. *)
+
+Program Definition interpTMem n
+        (A1 : type_dom n)
+        (A2 : type_dom n)
+        (val_type2 : ty -> list vl -> list vl -> vl -> forall j, j < n -> Prop) :=
+  fun env GH v n0 (p : n0 <= n) =>
+    match v with
+    | vty env1 TX =>
+      forall j (Hj : j < n0),
+      forall vy,
+        (A1 env GH vy j _ -> val_type2 TX env1 GH vy j _) /\
+        (val_type2 TX env1 GH vy j _ -> A2 env GH vy j _)
+    | _ => False
+    end.
+
+Program Fixpoint val_type2 (T: ty) (env: list vl) (GH: list vl) (v:vl)
+        (n: nat) {measure (val_type_measure T n) (termRel)}: Prop :=
+  match T with
+    | TAll T1 T2 =>
+      closed 0 (length GH) (length env) T1 /\ closed 1 (length GH) (length env) T2 /\
+      interpTAll n
+                 (* (val_type2 T1) *)
+                 (conv val_type2 T1 _)
+                 (* (fun env GH v n p => *)
+                 (*    val_type2 T1 *)
+                 (*              env GH v n) *)
+                 (conv val_type2 (open (varH (length GH)) T2) _)
+                 (* (fun env GH v n p => *)
+                 (*    val_type2 *)
+                 (*      (open (varH (length GH)) T2) *)
+                 (*              env GH v n) *)
+                 env GH v n _
+    | TMem T1 T2 =>
+      closed 0 (length GH) (length env) T1 /\ closed 0 (length GH) (length env) T2 /\
+      interpTMem n
+                 (conv val_type2 T1 _)
+                 (conv val_type2 T2 _)
+                 (fun T GH env v j p => val_type2 T GH env v j)
+                 GH env v n _
+      (* match v with *)
+      (* | vty env1 TX => *)
+      (*   forall j (Hj : j < n), *)
+      (*   forall vy, *)
+      (*     (val_type2 T1 env GH vy j -> val_type2 TX env1 GH vy j) /\ *)
+      (*     (val_type2 TX env1 GH vy j -> val_type2 T2 env GH vy j) *)
+      (* | _ => False *)
+      (* end *)
+    | _ =>
+      False
+  end.
+
+(* Solve Obligations with valTypeObligationsSSReflection. *)
+
+Axiom prop_extensionality:
+  forall (P Q: Prop), (P <-> Q) -> P = Q.
+
+(* this is just to accelerate Coq -- val_type in the goal is slooow *)
+Inductive vtp2: ty -> list vl -> list vl -> vl -> forall n, Prop :=
+| vv2: forall T G H n v, val_type2 T G H v n -> vtp2 T G H v n.
+
+Lemma unvv2: forall T G H v n,
+  vtp2 T G H v n -> val_type2 T G H v n.
+Proof.
+  intros * H0. destruct H0. assumption.
+Qed.
+
+Lemma vtp2_unfold: forall T G H v n,
+  vtp2 T G H v n = val_type2 T G H v n.
+Proof.
+  intros.
+  apply prop_extensionality.
+  split; intros.
+  - apply unvv2. assumption.
+  - constructor. assumption.
+Qed.
+
+Lemma vtp2_unfold':
+  vtp2 = val_type2.
+Proof.
+  repeat (apply functional_extensionality; intro).
+  apply vtp2_unfold.
+Qed.
+
+(*
+   The expansion of val_type, val_type_func is incomprehensible.
+   We cannot (easily) unfold and reason about it. Therefore, we prove unfolding of
+   val_type to its body as a lemma.
+   (Note that the unfold_sub tactic relies on
+   functional extensionality)
+*)
+
+(* Triggers anomaly: *)
+(* Program Definition conv2 n (A: ty -> list vl -> list vl -> vl -> nat -> Prop) T1: *)
+(*   list vl -> list vl -> vl -> forall (n0 : nat) (H : n0 <= n), Prop := *)
+(*    fun env GH v n p => A T1 env GH v n. *)
+
+(* Program Lemma val_type2_unfold' : forall T env GH v n, *)
+(*     val_type2 T env GH v n = *)
+(*     match T with *)
+(*     | TAll T1 T2 => *)
+(*       closed 0 (length GH) (length env) T1 /\ closed 1 (length GH) (length env) T2 /\ *)
+(*       interpTAll n *)
+(*                  (* (val_type2 T1) *) *)
+(*                  (* (val_type2 T1) *) *)
+(*                  (conv2 val_type2 T1) *)
+(*                  (* (fun env GH v n p => *) *)
+(*                  (*    val_type2 T1 *) *)
+(*                  (*              env GH v n) *) *)
+(*                  (conv2 val_type2 (open (varH (length GH)) T2)) *)
+(*                  (* (fun env GH v n p => *) *)
+(*                  (*    val_type2 *) *)
+(*                  (*      (open (varH (length GH)) T2) *) *)
+(*                  (*              env GH v n) *) *)
+(*                  env GH v n _ *)
+(*     | _ => *)
+(*       False *)
+(*     end. *)
+
+
+
+Program Definition conv2 n (A: ty -> list vl -> list vl -> vl -> nat -> Prop) T1:
+  list vl -> list vl -> vl -> forall (n0 : nat) (H : n0 <= n), Prop :=
+   fun env GH v n p => A T1 env GH v n.
+
+(* Lemma val_type2_unfold' : forall T env GH v n, *)
+(*     val_type2 T env GH v n = *)
+(*     match T with *)
+(*     | TAll T1 T2 => *)
+(*       closed 0 (length GH) (length env) T1 /\ closed 1 (length GH) (length env) T2 /\  *)
+(*       interpTAll n *)
+(*                  (* (val_type2 T1) *) *)
+(*                  (* (val_type2 T1) *) *)
+(*                  (@conv2 n val_type2 T1) *)
+(*                  (* (fun env GH v n p => *) *)
+(*                  (*    val_type2 T1 *) *)
+(*                  (*              env GH v n) *) *)
+(*                  (@conv2 n val_type2 (open (varH (length GH)) T2)) *)
+(*                  (* (fun env GH v n p => *) *)
+(*                  (*    val_type2 *) *)
+(*                  (*      (open (varH (length GH)) T2) *) *)
+(*                  (*              env GH v n) *) *)
+(*                  env GH v n (le_n _) *)
+(*     | _ => *)
+(*       False *)
+(*     end. *)
+(* Proof. *)
+(*   intros. unfold val_type2 at 1; unfold val_type2_func; *)
+(*   unfold_sub val_type2 (val_type2 T env GH v n); *)
+(*   program_simplify; *)
+(*   repeat (norepeat_match_case_analysis_goal; try reflexivity). *)
+(* Qed. *)
+
 (*
 Again:
 The first env (env, or G1) is for looking up varF variables.
@@ -94,92 +371,22 @@ Program Fixpoint val_type (env: list vl) (GH: list vl) (T:ty) (n: nat) (v:vl)
 
     | _, TAnd T1 T2 =>
       val_type env GH T1 n v /\ val_type env GH T2 n v
-        
+
     | _, TBind T1 =>
       closed 1 (length GH) (length env) T1 /\
       val_type env (v::GH) (open (varH (length GH)) T1) n v
-                                  
+
     | _, TTop =>
       True
     | _,_ =>
       False
   end.
-
-(* Show that different branches are disjoint. *)
-Ltac discriminatePlus := repeat split; intros; let Habs := fresh "Habs" in intro Habs; destruct Habs; discriminate.
-
-(* Prove some inequalities needed below, without producing big proof terms like omega does. Probably not worth it. *)
-Ltac simple_ineq :=
-  (* simpl; omega. *)
-  simpl; auto using le_n_S, le_plus_l, le_plus_r.
-  (* If this tactic fails, add back omega at the end. *)
-
-(* These three lemmas take care of the various forms of proof obligations that arise from val_type. *)
-Lemma termRelShow: forall j n T1 T2,
-  j <= n -> tsize_flat T2 < tsize_flat T1 ->
-  val_type_termRel (T2, j) (T1, n).
-Proof.
-  intros * Hj Ht.
-  unfold val_type_termRel, MR, termRel, argMeasure, val_type_measure.
-  (* If we only know that Hj: j <= n, we must case-split on it, and use
-     smaller_types when j = n and smaller_n when j < n. *)
-  destruct Hj; try assert (j < S m) by simple_ineq; auto using left_lex, right_lex.
-Qed.
-  (* - apply right_lex. assumption. *)
-  (* - apply left_lex. omega. *)
-
-
-Lemma termRelShowOpen: forall j n x T1 T2,
-  j <= n -> tsize_flat T2 < tsize_flat T1 ->
-  val_type_termRel (open (varH x) T2, j) (T1, n).
-Proof.
-  intros * Hj Ht.
-  unfold val_type_termRel, MR, termRel, argMeasure, val_type_measure.
-  destruct Hj; try assert (j < S m) by simple_ineq; auto using left_lex, right_lex.
-  unfold open; try rewrite <- open_preserves_size.
-  auto using left_lex, right_lex.
-Qed.
-
-Lemma termRelShowLt: forall j n T1 T2,
-  j < n ->
-  val_type_termRel (T2, j) (T1, n).
-Proof.
-  intros * Hj.
-  unfold val_type_termRel, MR, termRel, argMeasure, val_type_measure.
-  auto using left_lex, right_lex.
-Qed.
-
-Ltac applyNSimpleIneq l := apply l; simple_ineq.
-
-(* Solve obligations from valType using ssreflect-based ideas, that is, reusing lemmas for the various cases. *)
-Ltac valTypeObligationsSSReflection :=
-  program_simpl;
-  solve [applyNSimpleIneq termRelShowOpen | applyNSimpleIneq termRelShow | applyNSimpleIneq termRelShowLt | discriminatePlus].
-
-Ltac smaller_n :=
-  Tactics.program_simpl;
-  autounfold; apply left_lex;
-  (* simpl; omega. *)
-  simple_ineq.
-
-Ltac smaller_types :=
-  Tactics.program_simpl;
-  autounfold; apply right_lex;
-  unfold open; try rewrite <- open_preserves_size;
-  (* simpl; omega. *)
-  simple_ineq.
-
-Ltac valTypeObligations Hj :=
-  Tactics.program_simpl;
-  solve [ smaller_n | smaller_types | discriminatePlus | (try destruct Hj; [ smaller_types | smaller_n ])].
-
-
 (* Broken *)
 (* Ltac valTypeObligationsOld := *)
 (*   Tactics.program_simpl; *)
 (*   smaller_n || smaller_types || discriminatePlus || *)
 (*             (apply termRelShowOpen || apply termRelShow || apply termRelShowLt); auto; *)
-(*   unfold open; try rewrite <- open_preserves_size; *)
+(*   unfold open; try rewrite open_preserves_size'; *)
 (*   (* simple_ineq. *) *)
 (*   simpl; omega. *)
 
@@ -189,7 +396,7 @@ Ltac valTypeObligations Hj :=
 (* Solve Obligations with valTypeObligations Hj. *)
 
 (* Better *)
-Solve Obligations with valTypeObligationsSSReflection.
+(* Solve Obligations with valTypeObligationsSSReflection. *)
 
 (* this is just to accelerate Coq -- val_type in the goal is slooow *)
 Inductive vtp: list vl -> list vl -> ty -> forall n, vl -> Prop :=
@@ -201,16 +408,14 @@ Proof.
   intros * H0. destruct H0. assumption.
 Qed.
 
-Axiom prop_extensionality:
-  forall (P Q: Prop), (P <-> Q) -> P = Q.
 Lemma vtp_unfold: forall G H T n v,
   vtp G H T n v = val_type G H T n v.
 Proof.
   intros.
   apply prop_extensionality.
   split; intros.
-  apply unvv. assumption.
-  constructor. assumption.
+  - apply unvv. assumption.
+  - constructor. assumption.
 Qed.
 
 Lemma vtp_unfold':
@@ -220,11 +425,11 @@ Proof.
   apply vtp_unfold.
 Qed.
 
-(* 
-   The expansion of val_type, val_type_func is incomprehensible. 
+(*
+   The expansion of val_type, val_type_func is incomprehensible.
    We cannot (easily) unfold and reason about it. Therefore, we prove unfolding of
    val_type to its body as a lemma.
-   (Note that the unfold_sub tactic relies on 
+   (Note that the unfold_sub tactic relies on
    functional extensionality)
 *)
 
